prefix xsd: <http://www.w3.org/2001/XMLSchema#>
prefix rdf: <http://www.w3.org/1999/02/22-rdf-syntax-ns#>
prefix rdfs: <http://www.w3.org/2000/01/rdf-schema#>
prefix cc: <http://creativecommons.org/ns#>
prefix dcterms: <http://purl.org/dc/terms/>
prefix owl: <http://www.w3.org/2002/07/owl#>
prefix schema:   <http://schema.org/>
prefix vann: <http://purl.org/vocab/vann/>
prefix vcard: <http://www.w3.org/2006/vcard/ns#>
prefix gen: <http://www.w3.org/2006/gen/ont#>
prefix acp: <http://www.w3.org/ns/solid/acp#>


acp: a owl:Ontology ;
    owl:versionInfo "0.1" ;
    dcterms:title "Solid Access Change Policy Vocabulary"@en ;
    dcterms:description "A vocabulary to structure policy-based access changes for the Solid ecosystem."@en ;
    dcterms:creator <https://inrupt.com/profile/card/#us> ;
    dcterms:issued "2020-09-15"^^xsd:date ;
    vann:preferredNamespacePrefix "acp" ;
    vann:preferredNamespaceUri "http://www.w3.org/ns/solid/acp#" ;
    cc:attributionURL acp: ;
    cc:license <https://creativecommons.org/publicdomain/zero/1.0/> .

########################
#   Named Individuals
########################

acp:AuthenticatedAgent a rdfs:Resource ;
    rdfs:label "Authenticated Agent"@en ;
    rdfs:comment """An IRI representing an authenticated agent.
 Please note that in a decentralized authentication ecosystem, an authenticated agent may be ephemeral
 and, from a security standpoint, may not be significantly different than an anonymous agent"""@en ;
    rdfs:isDefinedBy acp: .

acp:CreatorAgent a rdfs:Resource ;
    rdfs:label "Creator Agent"@en ;
    rdfs:comment "An IRI representing the creator of a resource."@en ;
    rdfs:isDefinedBy acp: .

acp:PublicAgent a rdfs:Resource ;
    rdfs:label "Public Agent"@en ;
    rdfs:comment "An IRI representing a public or anonymous agent"@en ;
    rdfs:isDefinedBy acp: .


#################
#   Classes
#################

acp:AccessChange a rdfs:Class ;
    rdfs:label "Access Change"@en ;
    rdfs:comment "Access Change statements associate an AccessChangeResource with specific Policy definitions."@en ;
    rdfs:isDefinedBy acp: .

acp:AccessChangeResource a rdfs:Class ;
    rdfs:label "Access Change Resource"@en ;
    rdfs:comment "An RDF resource that includes AccessChange statements"@en ;
    rdfs:isDefinedBy acp: .

acp:Policy a rdfs:Class ;
    rdfs:label "Access Policy"@en ;
    rdfs:comment "A Policy defines a collection of access modes along with the conditions under which the policy is applied."@en ;
    rdfs:isDefinedBy acp: .

acp:Rule a rdfs:Class ;
    rdfs:label "Rule"@en ;
    rdfs:comment "A Rule defines which agent(s), group(s) and client application(s) match a Policy filter"@en ;
    rdfs:isDefinedBy acp: .

acp:AccessMode a rdfs:Class ;
    rdfs:label "Access Mode"@en ;
    rdfs:comment "An abstract access mode. This class should not be used directly. Instead, please use Read, Write and Append"@en ;
    rdfs:isDefinedBy acp: .

acp:Read a rdfs:Class ;
    rdfs:label "Read"@en ;
    rdfs:comment "An access mode indicating Read access"@en ;
    rdfs:subClassOf acp:AccessMode ;
    rdfs:isDefinedBy acp: .

acp:Write a rdfs:Class ;
    rdfs:label "Write"@en ;
    rdfs:comment "An access mode indicating Write access"@en ;
    rdfs:subClassOf acp:AccessMode ;
    rdfs:isDefinedBy acp: .

acp:Append a rdfs:Class ;
    rdfs:label "Append"@en ;
    rdfs:comment "An access mode indicating Append access. Append is a more limited form of Write in which data may only be added but not removed."@en ;
    rdfs:subClassOf acp:AccessMode ;
    rdfs:isDefinedBy acp: .


####################
#   Properties
####################

acp:accessChange a rdf:Property ;
    rdfs:label "accessChange"@en ;
    rdfs:comment """The object of this relationship is the access change resource associated with the subject resource.
 This relationship is intended to be used as the rel type of a Link, via HTTP Link Headers rfc5988 for Linked Data resources."""@en ;
    rdfs:domain gen:InformationResource ;
    rdfs:range acp:AccessChangeResource;
    rdfs:isDefinedBy acp: .

acp:access a rdf:Property ;
    rdfs:label "access"@en ;
    rdfs:comment "The access property identifies the access policies that apply to the ACR itself."@en ;
    rdfs:range acp:Policy ;
    rdfs:isDefinedBy acp: .

acp:accessLocked a rdf:Property ;
    rdfs:label "access locked"@en ;
    rdfs:comment """The accessLocked property identifies the access policies that apply to the ACR itself.
 These policies may not be removed except by an agent with write access to the root ACR."""@en ;
    rdfs:range acp:Policy ;
    rdfs:isDefinedBy acp: .

acp:accessProtected a rdf:Property ;
    rdfs:label "access protected"@en ;
    rdfs:comment """The accessProtected property identifies the access policies that apply to the ACR itself.
 These policies may not be removed except by an agent with write access to the ACR where the policy was initially applied."""@en ;
    rdfs:range acp:Policy ;
    rdfs:isDefinedBy acp: .

acp:accessMembers a rdf:Property ;
    rdfs:label "access members"@en ;
    rdfs:comment "The accessMembers property identifies the access policies that apply to the ACR itself, recursively."@en ;
    rdfs:range acp:Policy ;
    rdfs:isDefinedBy acp: .

acp:accessMembersLocked a rdf:Property ;
    rdfs:label "access members locked"@en ;
    rdfs:comment """The accessMembersLocked property identifies the access policies that apply to the ACR itself, recursively.
    These policies may not be removed except by an agent with write access to the root ACR."""@en ;
    rdfs:range acp:Policy ;
    rdfs:isDefinedBy acp: .

acp:accessMembersProtected a rdf:Property ;
    rdfs:label "access members protected"@en ;
    rdfs:comment """The accessMembersProtected property identifies the access policies that apply to the ACR itself, recursively.
    These policies may not be removed except by an agent with write access to the ACR where the policy was initially applied."""@en ;
    rdfs:range acp:Policy ;
    rdfs:isDefinedBy acp: .

acp:apply a rdf:Property ;
    rdfs:label "apply"@en ;
    rdfs:comment "The apply property indentifies the access policies to apply to a resource."@en ;
    rdfs:domain acp:AccessChange ;
    rdfs:range acp:Policy ;
    rdfs:isDefinedBy acp: .

acp:applyProtected a rdf:Property ;
    rdfs:label "apply protected"@en ;
    rdfs:comment """The applyProtected property identifies the access policies to apply to a resource's members recursively.
    These policies may not be removed except by an agent with write access to the ACR where the policy was initially applied."""@en ;
    rdfs:domain acp:AccessChange ;
    rdfs:range acp:Policy ;
    rdfs:isDefinedBy acp: .

acp:applyLocked a rdf:Property ;
    rdfs:label "apply locked"@en ;
    rdfs:comment """The applyLocked property identifies the access policies to apply to a resource's members recursively.
 These policies may not be removed except by an agent with write access to the root ACR."""@en ;
    rdfs:domain acp:AccessChange ;
    rdfs:range acp:Policy ;
    rdfs:isDefinedBy acp: .

acp:applyMembers a rdf:Property ;
    rdfs:label "apply members"@en ;
    rdfs:comment "The applyMembers property indentifies the access policies to apply to a resource's members recursively."@en ;
    rdfs:domain acp:AccessChange ;
    rdfs:range acp:Policy ;
    rdfs:isDefinedBy acp: .

acp:applyMembersProtected a rdf:Property ;
    rdfs:label "apply members protected"@en ;
    rdfs:comment """The applyMembersProtected property identifies the access policies to apply to a resource's members recursively.
 These policies may not be removed except by an agent with write access to the ACR where the policy was initially applied."""@en ;
    rdfs:domain acp:AccessChange ;
    rdfs:range acp:Policy ;
    rdfs:isDefinedBy acp: .

acp:applyMembersLocked a rdf:Property ;
    rdfs:label "apply members locked"@en ;
    rdfs:comment """The applyMembersLocked property identifies the access policies to apply to a resource's members recurseively.
 These policies may not be removed except by an agent with write access to the root ACR."""@en ;
    rdfs:domain acp:AccessChange ;
    rdfs:range acp:Policy ;
    rdfs:isDefinedBy acp: .

acp:allOf a rdf:Property ;
    rdfs:label "all of"@en ;
    rdfs:comment "The allOf property identifies a collection of Rules, each of which must match in order for the Policy to take effect."@en ;
    rdfs:domain acp:Policy ;
    rdfs:range acp:Rule ;
    rdfs:isDefinedBy acp: .

acp:anyOf a rdf:Property ;
    rdfs:label "any of"@en ;
    rdfs:comment "The anyOf property identifies a collection of Rules, one of which must match in order for the Policy to take effect."@en ;
    rdfs:domain acp:Policy ;
    rdfs:range acp:Rule ;
    rdfs:isDefinedBy acp: .

acp:noneOf a rdf:Property ;
    rdfs:label "none of"@en ;
    rdfs:comment "The noneOf property identifies a collection of Rules, none of which must match in order for the Policy to take effect."@en ;
    rdfs:domain acp:Policy ;
    rdfs:range acp:Rule ;
    rdfs:isDefinedBy acp: .

acp:allow a rdf:Property ;
    rdfs:label "allow"@en ;
    rdfs:comment "The allow property identifies the access modes a Policy allows."@en ;
    rdfs:domain acp:Policy ;
    rdfs:range acp:AccessMode ;
    rdfs:isDefinedBy acp: .

acp:deny a rdf:Property ;
    rdfs:label "deny"@en ;
    rdfs:comment "The deny property identifies the access modes a Policy denies."@en ;
    rdfs:domain acp:Policy ;
    rdfs:range acp:AccessMode ;
    rdfs:isDefinedBy acp: .

acp:agent a rdf:Property ;
    rdfs:label "agent"@en ;
    rdfs:comment "The agent property identifies the agent WebID(s) to which a Rule applies."@en ;
    rdfs:domain acp:Rule ;
    rdfs:isDefinedBy acp: .

acp:client a rdf:Property ;
    rdfs:label "client"@en ;
    rdfs:comment "The client property identifies the client WebID(s) to which a Rule applies."@en ;
    rdfs:domain acp:Rule ;
    rdfs:isDefinedBy acp: .

acp:group a rdf:Property ;
    rdfs:label "group"@en ;
    rdfs:comment "The group property identifies the vcard group(s) to which a Rule applies."@en ;
    rdfs:domain acp:Rule ;
    rdfs:range vcard:Group ;
    rdfs:isDefinedBy acp: .
